scheduler/SchA.v
@@ -235,21 +235,23 @@ Module SchAS. Section SchAS.
   Section SPEC.
 
     (* TODO : clarify with WP tc *)
-    Definition fspec_spawnable (u : univ_id) (fsp : fspec) (tid: nat) (m : meta fsp)
-        (vargs args : Any.t) (pre : iProp Σ) (postS: SAny.t -> SynDepO) : Prop :=
-      (((wsim_ginv u ⊤) ∗ (tid_user tid) ∗ pre ⊢ (precond fsp m vargs args))%I ∧
-      (∀ ret: Any.t, 
-        ((∃ vret, postcond fsp m vret ret)%I ⊢
-          ((wsim_ginv u ⊤) ∗ (tid_user tid) ∗ ∃ sret: SAny.t, (⌜ret = sret↑⌝ ∗ interp_cond (postS sret))))%I)).
+    Definition fspec_spawnable (u : univ_id) (fsp : fspec)
+        (pre : iProp Σ) (postS: SAny.t -> SynDepO) : Prop :=
+      fspec_weaker
+        (w_fspec u (fspec_simple (λ tid : nat,
+          ((λ _, tid_user tid ∗ pre)%I,
+          (λ ret, tid_user tid ∗ ∃ sret: SAny.t, (⌜ret = sret↑⌝ ∗ interp_cond (postS sret)))%I)
+          )))
+        fsp.
 
     Definition _spawn_spec : fspec := 
       w_fspec υ
         (fspec_virtual
-          (λ '(my_tid, pa_tid, fargs, fvargs, pre, postS, existT fn m) varg arg,
+          (λ '(my_tid, pa_tid, fargs, fvargs, pre, postS, fn) varg arg,
             (⌜varg = ((pa_tid, fn, fvargs) : nat * string * SAny.t) 
               ∧ arg = ((pa_tid, fn, fargs) : nat * string * SAny.t)↑ 
               ∧ is_Some (Spc_user fn)
-              ∧ fspec_spawnable υ (find_fsp Spc_user fn) my_tid m fvargs↑ fargs↑ pre postS⌝
+              ∧ fspec_spawnable υ (find_fsp Spc_user fn) pre postS⌝
             ∗ pre ∗ (token_half my_tid postS) ∗ (tid_user my_tid))%I)
           (λ _ (_: SAny.t) _, (False)%I))
     .
@@ -257,13 +259,13 @@ Module SchAS. Section SchAS.
     Definition spawn_spec : fspec :=
       w_fspec υ
         (fspec_virtual
-          (λ '(my_tid, fargs, fvargs, pre, postS, existT fn m) varg arg,
+          (λ '(my_tid, fargs, fvargs, pre, postS, fn) varg arg,
             (⌜varg = ((fn, fvargs): string * SAny.t) 
               ∧ arg = ((fn, fargs): string * SAny.t)↑
               ∧ is_Some (Spc_user fn)
-              ∧ (∀ tid, fspec_spawnable υ (find_fsp Spc_user fn) tid m fvargs↑ fargs↑ pre postS)⌝
+              ∧ (fspec_spawnable υ (find_fsp Spc_user fn) pre postS)⌝
              ∗ pre ∗ tid_user my_tid)%I)
-          (fun '(my_tid, fargs, fvargs, pre, postS, existT fn m) vret ret => 
+          (λ '(my_tid, fargs, fvargs, pre, postS, fn) vret ret,
             ((∃ tid: nat, ⌜vret = tid ∧ ret = tid↑⌝ ∗ (token_th tid postS)) ∗ tid_user my_tid)%I))
     .
 
